

CS 228 : Logic in Computer Science

Krishna. S

Completeness

$$\varphi_1, \dots, \varphi_n \models \psi \Rightarrow \varphi_1, \dots, \varphi_n \vdash \psi$$

Whenever $\varphi_1, \dots, \varphi_n$ semantically entail ψ , then ψ can be proved from $\varphi_1, \dots, \varphi_n$. The proof rules are **complete**

Completeness : 3 steps

- ▶ Given $\varphi_1, \dots, \varphi_n \models \psi$
- ▶ Step 1: Show that $\models \varphi_1 \rightarrow (\varphi_2 \rightarrow (\dots (\varphi_n \rightarrow \psi) \dots))$
- ▶ Step 2: Show that $\vdash \varphi_1 \rightarrow (\varphi_2 \rightarrow (\dots (\varphi_n \rightarrow \psi) \dots))$
- ▶ Step 3: Show that $\varphi_1, \dots, \varphi_n \vdash \psi$

Completeness : Step 1

- ▶ Assume $\varphi_1, \dots, \varphi_n \models \psi$. Whenever all of $\varphi_1, \dots, \varphi_n$ evaluate to true, so does ψ .
- ▶ If $\not\models \varphi_1 \rightarrow (\varphi_2 \rightarrow (\dots (\varphi_n \rightarrow \psi) \dots))$, then ψ evaluates to false when all of $\varphi_1, \dots, \varphi_n$ evaluate to true, a contradiction.
- ▶ Hence, $\models \varphi_1 \rightarrow (\varphi_2 \rightarrow (\dots (\varphi_n \rightarrow \psi) \dots))$.

Completeness : Step 2

- ▶ Given $\models \psi$, show that $\vdash \psi$
- ▶ Assume p_1, \dots, p_n are the propositional variables in ψ . We know that all the 2^n assignments of values to p_1, \dots, p_n make ψ true.
- ▶ Using this insight, we have to give a proof of ψ .

Completeness : Step 2

Truth Table to Proof

Let φ be a formula with variables p_1, \dots, p_n . Let \mathcal{T} be the truth table of φ , and let l be a line number in \mathcal{T} . Let \hat{p}_i represent p_i if p_i is assigned true in line l , and let it denote $\neg p_i$ if p_i is assigned false in line l . Then

1. $\hat{p}_1, \dots, \hat{p}_n \vdash \varphi$ if φ evaluates to true in line l
2. $\hat{p}_1, \dots, \hat{p}_n \vdash \neg\varphi$ if φ evaluates to false in line l

Truth Table to Proof

- ▶ Structural Induction on φ . Induct on the size of the formula, and do a case analysis.

Truth Table to Proof

- ▶ Structural Induction on φ . Induct on the size of the formula, and do a case analysis.
- ▶ Size of the formula = 1 + height of the parse tree
What is a parse tree?

Truth Table to Proof

- ▶ Structural Induction on φ . Induct on the size of the formula, and do a case analysis.
- ▶ Size of the formula = 1 + height of the parse tree
What is a parse tree?
- ▶ Base : If $\varphi = p$, a proposition, with size 1. In this case, $p \vdash p$ and $\neg p \vdash \neg p$, and we are done.

Truth Table to Proof

- ▶ Structural Induction on φ . Induct on the size of the formula, and do a case analysis.
- ▶ Size of the formula = 1 + height of the parse tree
What is a parse tree?
- ▶ Base : If $\varphi = p$, a proposition, with size 1. In this case, $p \vdash p$ and $\neg p \vdash \neg p$, and we are done.
- ▶ Assume for formulae of size $\leq k - 1$

Truth Table to Proof

- ▶ Structural Induction on φ . Induct on the size of the formula, and do a case analysis.
- ▶ Size of the formula = 1 + height of the parse tree
What is a parse tree?
- ▶ Base : If $\varphi = p$, a proposition, with size 1. In this case, $p \vdash p$ and $\neg p \vdash \neg p$, and we are done.
- ▶ Assume for formulae of size $\leq k - 1$
- ▶ Case Negation : $\varphi = \neg\varphi_1$. The inductive hypothesis applies to φ_1 .

Truth Table to Proof

- ▶ Structural Induction on φ . Induct on the size of the formula, and do a case analysis.
- ▶ Size of the formula = 1 + height of the parse tree
What is a parse tree?
- ▶ Base : If $\varphi = p$, a proposition, with size 1. In this case, $p \vdash p$ and $\neg p \vdash \neg p$, and we are done.
- ▶ Assume for formulae of size $\leq k - 1$
- ▶ Case Negation : $\varphi = \neg\varphi_1$. The inductive hypothesis applies to φ_1 .
 - ▶ Assume φ evaluates to true in line l of \mathcal{T} . Then φ_1 evaluates to false in line l . By inductive hypothesis, $\hat{p}_1, \dots, \hat{p}_n \vdash \neg\varphi_1$.

Truth Table to Proof

- ▶ Structural Induction on φ . Induct on the size of the formula, and do a case analysis.
- ▶ Size of the formula = 1 + height of the parse tree
What is a parse tree?
- ▶ Base : If $\varphi = p$, a proposition, with size 1. In this case, $p \vdash p$ and $\neg p \vdash \neg p$, and we are done.
- ▶ Assume for formulae of size $\leq k - 1$
- ▶ Case Negation : $\varphi = \neg\varphi_1$. The inductive hypothesis applies to φ_1 .
 - ▶ Assume φ evaluates to true in line l of \mathcal{T} . Then φ_1 evaluates to false in line l . By inductive hypothesis, $\hat{p}_1, \dots, \hat{p}_n \vdash \neg\varphi_1$.
 - ▶ Assume φ evaluates to false in line l of \mathcal{T} . Then φ_1 evaluates to true in line l . By inductive hypothesis, $\hat{p}_1, \dots, \hat{p}_n \vdash \varphi_1$.

Truth Table to Proof

- ▶ Structural Induction on φ . Induct on the size of the formula, and do a case analysis.
- ▶ Size of the formula = 1 + height of the parse tree
What is a parse tree?
- ▶ Base : If $\varphi = p$, a proposition, with size 1. In this case, $p \vdash p$ and $\neg p \vdash \neg p$, and we are done.
- ▶ Assume for formulae of size $\leq k - 1$
- ▶ Case Negation : $\varphi = \neg\varphi_1$. The inductive hypothesis applies to φ_1 .
 - ▶ Assume φ evaluates to true in line l of \mathcal{T} . Then φ_1 evaluates to false in line l . By inductive hypothesis, $\hat{p}_1, \dots, \hat{p}_n \vdash \neg\varphi_1$.
 - ▶ Assume φ evaluates to false in line l of \mathcal{T} . Then φ_1 evaluates to true in line l . By inductive hypothesis, $\hat{p}_1, \dots, \hat{p}_n \vdash \varphi_1$.
 - ▶ Use the $\neg i$ rule to obtain a proof of $\hat{p}_1, \dots, \hat{p}_n \vdash \neg\neg\varphi_1$.

Truth Table to Proof

- ▶ Case \rightarrow : $\varphi = \varphi_1 \rightarrow \varphi_2$.

Truth Table to Proof

- ▶ Case \rightarrow : $\varphi = \varphi_1 \rightarrow \varphi_2$.
 - ▶ If φ evaluates to false in line l , then φ_1 evaluates to true and φ_2 to false. Let $\{q_1, \dots, q_k\}$ be the variables of φ_1 and let $\{r_1, \dots, r_j\}$ be the variables in φ_2 . $\{q_1, \dots, q_k\} \cup \{r_1, \dots, r_j\} = \{p_1, \dots, p_n\}$.

Truth Table to Proof

- ▶ Case \rightarrow : $\varphi = \varphi_1 \rightarrow \varphi_2$.
 - ▶ If φ evaluates to false in line l , then φ_1 evaluates to true and φ_2 to false. Let $\{q_1, \dots, q_k\}$ be the variables of φ_1 and let $\{r_1, \dots, r_j\}$ be the variables in φ_2 . $\{q_1, \dots, q_k\} \cup \{r_1, \dots, r_j\} = \{p_1, \dots, p_n\}$.
 - ▶ By inductive hypothesis, $\hat{q}_1, \dots, \hat{q}_k \models \varphi_1$ and $\hat{r}_1, \dots, \hat{r}_j \models \neg\varphi_2$. Then, $\hat{p}_1, \dots, \hat{p}_n \models \varphi_1 \wedge \neg\varphi_2$.

Truth Table to Proof

- ▶ Case \rightarrow : $\varphi = \varphi_1 \rightarrow \varphi_2$.
 - ▶ If φ evaluates to false in line l , then φ_1 evaluates to true and φ_2 to false. Let $\{q_1, \dots, q_k\}$ be the variables of φ_1 and let $\{r_1, \dots, r_j\}$ be the variables in φ_2 . $\{q_1, \dots, q_k\} \cup \{r_1, \dots, r_j\} = \{p_1, \dots, p_n\}$.
 - ▶ By inductive hypothesis, $\hat{q}_1, \dots, \hat{q}_k \models \varphi_1$ and $\hat{r}_1, \dots, \hat{r}_j \models \neg\varphi_2$. Then, $\hat{p}_1, \dots, \hat{p}_n \models \varphi_1 \wedge \neg\varphi_2$.
 - ▶ Prove that $\varphi_1 \wedge \neg\varphi_2 \vdash \neg(\varphi_1 \rightarrow \varphi_2)$.

Truth Table to Proof

- ▶ Case \rightarrow : $\varphi = \varphi_1 \rightarrow \varphi_2$.

Truth Table to Proof

- ▶ Case \rightarrow : $\varphi = \varphi_1 \rightarrow \varphi_2$.
 - ▶ If φ evaluates to true in line l , then there are 3 possibilities. If both φ_1, φ_2 evaluate to true, then we have $\hat{p}_1, \dots, \hat{p}_n \models \varphi_1 \wedge \varphi_2$. Proving $\varphi_1 \wedge \varphi_2 \vdash \varphi_1 \rightarrow \varphi_2$, we are done.

Truth Table to Proof

- ▶ Case \rightarrow : $\varphi = \varphi_1 \rightarrow \varphi_2$.
 - ▶ If φ evaluates to true in line l , then there are 3 possibilities. If both φ_1, φ_2 evaluate to true, then we have $\hat{p}_1, \dots, \hat{p}_n \models \varphi_1 \wedge \varphi_2$. Proving $\varphi_1 \wedge \varphi_2 \vdash \varphi_1 \rightarrow \varphi_2$, we are done.
 - ▶ If both φ_1, φ_2 evaluate to false, then we have $\hat{p}_1, \dots, \hat{p}_n \models \neg\varphi_1 \wedge \neg\varphi_2$. Proving $\neg\varphi_1 \wedge \neg\varphi_2 \vdash \varphi_1 \rightarrow \varphi_2$, we are done.

Truth Table to Proof

- ▶ Case \rightarrow : $\varphi = \varphi_1 \rightarrow \varphi_2$.
 - ▶ If φ evaluates to true in line l , then there are 3 possibilities. If both φ_1, φ_2 evaluate to true, then we have $\hat{p}_1, \dots, \hat{p}_n \models \varphi_1 \wedge \varphi_2$. Proving $\varphi_1 \wedge \varphi_2 \vdash \varphi_1 \rightarrow \varphi_2$, we are done.
 - ▶ If both φ_1, φ_2 evaluate to false, then we have $\hat{p}_1, \dots, \hat{p}_n \models \neg\varphi_1 \wedge \neg\varphi_2$. Proving $\neg\varphi_1 \wedge \neg\varphi_2 \vdash \varphi_1 \rightarrow \varphi_2$, we are done.
 - ▶ Last, if φ_1 evaluates to false and φ_2 evaluates to true, then we have $\hat{p}_1, \dots, \hat{p}_n \models \neg\varphi_1 \wedge \varphi_2$. Proving $\neg\varphi_1 \wedge \varphi_2 \vdash \varphi_1 \rightarrow \varphi_2$, we are done.

Truth Table to Proof

- ▶ Prove the cases \wedge, \vee .

On An Example

We know $\models (p \wedge q) \rightarrow p$. Using this fact, show that $\vdash (p \wedge q) \rightarrow p$.

- ▶ $p, q \vdash (p \wedge q) \rightarrow p$
- ▶ $\neg p, q \vdash (p \wedge q) \rightarrow p$
- ▶ $p, \neg q \vdash (p \wedge q) \rightarrow p$
- ▶ $\neg p, \neg q \vdash (p \wedge q) \rightarrow p$

Now, combine the 4 proofs above to give a single proof for $\vdash (p \wedge q) \rightarrow p$.

Completeness : Steps 2, 3

- ▶ Step 2: From $\models \varphi_1 \rightarrow (\varphi_2 \rightarrow (\dots (\varphi_n \rightarrow \psi) \dots))$, use LEM on all the propositional variables of $\varphi_1, \dots, \varphi_n, \psi$ to obtain $\vdash \varphi_1 \rightarrow (\varphi_2 \rightarrow (\dots (\varphi_n \rightarrow \psi) \dots))$.

Completeness : Steps 2, 3

- ▶ Step 2: From $\models \varphi_1 \rightarrow (\varphi_2 \rightarrow (\dots (\varphi_n \rightarrow \psi) \dots))$, use LEM on all the propositional variables of $\varphi_1, \dots, \varphi_n, \psi$ to obtain $\vdash \varphi_1 \rightarrow (\varphi_2 \rightarrow (\dots (\varphi_n \rightarrow \psi) \dots))$.
- ▶ Step 3: Take the proof $\vdash \varphi_1 \rightarrow (\varphi_2 \rightarrow (\dots (\varphi_n \rightarrow \psi) \dots))$. This proof has n nested boxes, the i th box opening with the assumption φ_i . The last box closes with the last line ψ . Hence, the line immediately after the last box is $\varphi_n \rightarrow \psi$.

Completeness : Steps 2, 3

- ▶ Step 2: From $\models \varphi_1 \rightarrow (\varphi_2 \rightarrow (\dots (\varphi_n \rightarrow \psi) \dots))$, use LEM on all the propositional variables of $\varphi_1, \dots, \varphi_n, \psi$ to obtain $\vdash \varphi_1 \rightarrow (\varphi_2 \rightarrow (\dots (\varphi_n \rightarrow \psi) \dots))$.
- ▶ Step 3: Take the proof $\vdash \varphi_1 \rightarrow (\varphi_2 \rightarrow (\dots (\varphi_n \rightarrow \psi) \dots))$. This proof has n nested boxes, the i th box opening with the assumption φ_i . The last box closes with the last line ψ . Hence, the line immediately after the last box is $\varphi_n \rightarrow \psi$.
- ▶ In a similar way, the $(n - 1)$ th box has as its last line $\varphi_n \rightarrow \psi$, and hence, the line immediately after this box is $\varphi_{n-1} \rightarrow (\varphi_n \rightarrow \psi)$ and so on.

Completeness : Steps 2, 3

- ▶ Step 2: From $\models \varphi_1 \rightarrow (\varphi_2 \rightarrow (\dots (\varphi_n \rightarrow \psi) \dots))$, use LEM on all the propositional variables of $\varphi_1, \dots, \varphi_n, \psi$ to obtain $\vdash \varphi_1 \rightarrow (\varphi_2 \rightarrow (\dots (\varphi_n \rightarrow \psi) \dots))$.
- ▶ Step 3: Take the proof $\vdash \varphi_1 \rightarrow (\varphi_2 \rightarrow (\dots (\varphi_n \rightarrow \psi) \dots))$. This proof has n nested boxes, the i th box opening with the assumption φ_i . The last box closes with the last line ψ . Hence, the line immediately after the last box is $\varphi_n \rightarrow \psi$.
- ▶ In a similar way, the $(n - 1)$ th box has as its last line $\varphi_n \rightarrow \psi$, and hence, the line immediately after this box is $\varphi_{n-1} \rightarrow (\varphi_n \rightarrow \psi)$ and so on.
- ▶ Add premises $\varphi_1, \dots, \varphi_n$ on the top. Use MP on the premises, and the lines after boxes 1 to n in order to obtain ψ .

Summary

Propositional Logic is sound and complete.

Satisfiability and Validity

A formula φ over variables $\{p_1, \dots, p_n\}$ is satisfiable if there exists a valuation for p_1, \dots, p_n which makes φ true.

A formula φ over variables $\{p_1, \dots, p_n\}$ is unsatisfiable if there does not exist any valuation for p_1, \dots, p_n which makes φ true.

A formula φ over variables $\{p_1, \dots, p_n\}$ is valid if φ is true for all valuations to p_1, \dots, p_n .

Checking Satisfiability

- ▶ The SAT problem : Given a formula φ , is it satisfiable?
- ▶ Given a formula φ , is it valid?
- ▶ SAT is NP-complete. NP represents non-deterministic polynomial time.
- ▶ Given a witness, it is easy to check if the witness is a valid witness in polynomial time, Finding a witness is not as easy.
 - ▶ Given a valuation α for the variables p_1, \dots, p_n of a formula φ , we can check if φ evaluates to true under α in time polynomial in n .
 - ▶ Finding whether such a valuation α exists is not as easy.
- ▶ SAT solvers are tools which implement heuristics to check satisfiability.
- ▶ The input to a SAT solver is a formula in some specified form.

Normal Forms

- ▶ A **literal** is a propositional variable p or its negation $\neg p$. These are referred to as positive and negative literals respectively.

Normal Forms

- ▶ A **literal** is a propositional variable p or its negation $\neg p$. These are referred to as positive and negative literals respectively.
- ▶ A formula F is in Conjunctive Normal Form (CNF) if it is a conjunction of a disjunction of literals.

$$F = \bigwedge_{i=1}^n \bigvee_{j=1}^m L_{i,j}$$

each $L_{i,j}$ is a literal.

Normal Forms

- ▶ A **literal** is a propositional variable p or its negation $\neg p$. These are referred to as positive and negative literals respectively.
- ▶ A formula F is in Conjunctive Normal Form (CNF) if it is a conjunction of a disjunction of literals.

$$F = \bigwedge_{i=1}^n \bigvee_{j=1}^m L_{i,j}$$

each $L_{i,j}$ is a literal.

- ▶ A formula F is in DNF if it is a disjunction of a conjunction of literals.

$$F = \bigvee_{i=1}^n \bigwedge_{j=1}^m L_{i,j}$$

each $L_{i,j}$ is a literal.

Normal Forms

In the following, equivalent stands for semantically equivalent

Let F be a formula in CNF and let G be a formula in DNF. Then $\neg F$ is equivalent to a formula in DNF and $\neg G$ is equivalent to a formula in CNF.

Normal Forms

In the following, equivalent stands for semantically equivalent

Let F be a formula in CNF and let G be a formula in DNF. Then $\neg F$ is equivalent to a formula in DNF and $\neg G$ is equivalent to a formula in CNF.

Every formula F is equivalent to some formula F_1 in CNF and some formula F_2 in DNF.

CNF Algorithm

Given a formula F , ($x \rightarrow [\neg(y \vee z) \wedge \neg(y \rightarrow x)]$)

- ▶ Replace all subformulae of the form $F \rightarrow G$ with $\neg F \vee G$, and all subformulae of the form $F \leftrightarrow G$ with $(\neg F \vee G) \wedge (\neg G \vee F)$. When there are no more occurrences of $\rightarrow, \leftrightarrow$, proceed to the next step.

CNF Algorithm

Given a formula F , ($x \rightarrow [\neg(y \vee z) \wedge \neg(y \rightarrow x)]$)

- ▶ Replace all subformulae of the form $F \rightarrow G$ with $\neg F \vee G$, and all subformulae of the form $F \leftrightarrow G$ with $(\neg F \vee G) \wedge (\neg G \vee F)$. When there are no more occurrences of $\rightarrow, \leftrightarrow$, proceed to the next step.
- ▶ Get rid of all double negations : Replace all subformulae
 - ▶ $\neg\neg G$ with G ,
 - ▶ $\neg(G \wedge H)$ with $\neg G \vee \neg H$
 - ▶ $\neg(G \vee H)$ with $\neg G \wedge \neg H$

When there are no more such subformulae, proceed to the next step.

CNF Algorithm

Given a formula F , ($x \rightarrow [\neg(y \vee z) \wedge \neg(y \rightarrow x)]$)

- ▶ Replace all subformulae of the form $F \rightarrow G$ with $\neg F \vee G$, and all subformulae of the form $F \leftrightarrow G$ with $(\neg F \vee G) \wedge (\neg G \vee F)$. When there are no more occurrences of $\rightarrow, \leftrightarrow$, proceed to the next step.
- ▶ Get rid of all double negations : Replace all subformulae
 - ▶ $\neg\neg G$ with G ,
 - ▶ $\neg(G \wedge H)$ with $\neg G \vee \neg H$
 - ▶ $\neg(G \vee H)$ with $\neg G \wedge \neg H$

When there are no more such subformulae, proceed to the next step.

- ▶ Distribute \vee wherever possible.

The resultant formula F_1 is in CNF and is provably equivalent to F .

$$[(\neg x \vee \neg y) \wedge (\neg x \vee \neg z)] \wedge [(\neg x \vee y) \wedge (\neg x \vee \neg x)]$$

Polynomial Time Formula Classes

Horn Formulae

- ▶ A **Horn Formula** is a particularly nice kind of CNF formula, which can be **quickly** checked for satisfiability.
- ▶ Programming languages Prolog and Datalog are based on Horn clauses in first order logic

Horn Formulae

- ▶ A **Horn Formula** is a particularly nice kind of CNF formula, which can be **quickly** checked for satisfiability.
- ▶ Programming languages Prolog and Datalog are based on Horn clauses in first order logic
- ▶ A formula F is a Horn formula if it is in CNF and every disjunction contains at most one positive literal.

Horn Formulae

- ▶ A **Horn Formula** is a particularly nice kind of CNF formula, which can be **quickly** checked for satisfiability.
- ▶ Programming languages Prolog and Datalog are based on Horn clauses in first order logic
- ▶ A formula F is a Horn formula if it is in CNF and every disjunction contains at most one positive literal.
- ▶ $p \wedge (\neg p \vee \neg q \vee r) \wedge (\neg a \vee \neg b)$ is Horn, but $a \vee b$ is not Horn.

Horn Formulae

- ▶ A **Horn Formula** is a particularly nice kind of CNF formula, which can be **quickly** checked for satisfiability.
- ▶ Programming languages Prolog and Datalog are based on Horn clauses in first order logic
- ▶ A formula F is a Horn formula if it is in CNF and every disjunction contains at most one positive literal.
- ▶ $p \wedge (\neg p \vee \neg q \vee r) \wedge (\neg a \vee \neg b)$ is Horn, but $a \vee b$ is not Horn.
- ▶ A basic Horn formula is one which has no \wedge . Every Horn formula is a conjunction of basic Horn formulae.

Horn Formulae

- ▶ Three types of basic Horn : no positive literals, no negative literals, have both positive and negative literals.

Horn Formulae

- ▶ Three types of basic Horn : no positive literals, no negative literals, have both positive and negative literals.
- ▶ Basic Horn with both positive and negative literals are written as an implication $p \wedge q \wedge \cdots \wedge r \rightarrow s$ involving only positive literals.

Horn Formulae

- ▶ Three types of basic Horn : no positive literals, no negative literals, have both positive and negative literals.
- ▶ Basic Horn with both positive and negative literals are written as an implication $p \wedge q \wedge \cdots \wedge r \rightarrow s$ involving only positive literals.
- ▶ Basic Horn with no negative literals are of the form p and are written as $\top \rightarrow p$.

Horn Formulae

- ▶ Three types of basic Horn : no positive literals, no negative literals, have both positive and negative literals.
- ▶ Basic Horn with both positive and negative literals are written as an implication $p \wedge q \wedge \cdots \wedge r \rightarrow s$ involving only positive literals.
- ▶ Basic Horn with no negative literals are of the form p and are written as $\top \rightarrow p$.
- ▶ Basic Horn with no positive literals are written as $p \wedge q \wedge \cdots \wedge r \rightarrow \perp$.

Horn Formulae

- ▶ Three types of basic Horn : no positive literals, no negative literals, have both positive and negative literals.
- ▶ Basic Horn with both positive and negative literals are written as an implication $p \wedge q \wedge \cdots \wedge r \rightarrow s$ involving only positive literals.
- ▶ Basic Horn with no negative literals are of the form p and are written as $\top \rightarrow p$.
- ▶ Basic Horn with no positive literals are written as $p \wedge q \wedge \cdots \wedge r \rightarrow \perp$.
- ▶ Thus, a Horn formula is written as a conjunction of implications.

The Horn Algorithm

Given a Horn formula H ,

- ▶ Mark all occurrences of p , whenever $\top \rightarrow p$ is a subformula.

The Horn Algorithm

Given a Horn formula H ,

- ▶ Mark all occurrences of p , whenever $\top \rightarrow p$ is a subformula.
- ▶ If there is a subformula of the form $(p_1 \wedge \cdots \wedge p_m) \rightarrow q$, where each p_i is marked, and q is not marked, mark q . Repeat this until there are no subformulae of this form and proceed to the next step.

The Horn Algorithm

Given a Horn formula H ,

- ▶ Mark all occurrences of p , whenever $\top \rightarrow p$ is a subformula.
- ▶ If there is a subformula of the form $(p_1 \wedge \cdots \wedge p_m) \rightarrow q$, where each p_i is marked, and q is not marked, mark q . Repeat this until there are no subformulae of this form and proceed to the next step.
- ▶ Consider subformulae of the form $(p_1 \wedge \cdots \wedge p_m) \rightarrow \perp$. If there is one such subformula with all p_i marked, then say **Unsat**, otherwise say **Sat**.

An Example

$$(\top \rightarrow A) \wedge (C \rightarrow D) \wedge ((A \wedge B) \rightarrow C) \wedge ((C \wedge D) \rightarrow \perp) \wedge (\top \rightarrow B).$$

An Example

$$(\top \rightarrow A) \wedge (C \rightarrow D) \wedge ((A \wedge B) \rightarrow C) \wedge ((C \wedge D) \rightarrow \perp) \wedge (\top \rightarrow B).$$

► $(\top \rightarrow A) \wedge (C \rightarrow D) \wedge ((A \wedge B) \rightarrow C) \wedge ((C \wedge D) \rightarrow \perp) \wedge (\top \rightarrow B).$

An Example

$$(\top \rightarrow A) \wedge (C \rightarrow D) \wedge ((A \wedge B) \rightarrow C) \wedge ((C \wedge D) \rightarrow \perp) \wedge (\top \rightarrow B).$$

- ▶ $(\top \rightarrow A) \wedge (C \rightarrow D) \wedge ((A \wedge B) \rightarrow C) \wedge ((C \wedge D) \rightarrow \perp) \wedge (\top \rightarrow B).$
- ▶ $(\top \rightarrow A) \wedge (C \rightarrow D) \wedge ((A \wedge B) \rightarrow C) \wedge ((C \wedge D) \rightarrow \perp) \wedge (\top \rightarrow B).$

An Example

$$(\top \rightarrow A) \wedge (C \rightarrow D) \wedge ((A \wedge B) \rightarrow C) \wedge ((C \wedge D) \rightarrow \perp) \wedge (\top \rightarrow B).$$

- ▶ $(\top \rightarrow A) \wedge (C \rightarrow D) \wedge ((A \wedge B) \rightarrow C) \wedge ((C \wedge D) \rightarrow \perp) \wedge (\top \rightarrow B).$
- ▶ $(\top \rightarrow A) \wedge (C \rightarrow D) \wedge ((A \wedge B) \rightarrow C) \wedge ((C \wedge D) \rightarrow \perp) \wedge (\top \rightarrow B).$
- ▶ $(\top \rightarrow A) \wedge (C \rightarrow D) \wedge ((A \wedge B) \rightarrow C) \wedge ((C \wedge D) \rightarrow \perp) \wedge (\top \rightarrow B).$

An Example

$$(\top \rightarrow A) \wedge (C \rightarrow D) \wedge ((A \wedge B) \rightarrow C) \wedge ((C \wedge D) \rightarrow \perp) \wedge (\top \rightarrow B).$$

- ▶ $(\top \rightarrow A) \wedge (C \rightarrow D) \wedge ((A \wedge B) \rightarrow C) \wedge ((C \wedge D) \rightarrow \perp) \wedge (\top \rightarrow B).$
- ▶ $(\top \rightarrow A) \wedge (C \rightarrow D) \wedge ((A \wedge B) \rightarrow C) \wedge ((C \wedge D) \rightarrow \perp) \wedge (\top \rightarrow B).$
- ▶ $(\top \rightarrow A) \wedge (C \rightarrow D) \wedge ((A \wedge B) \rightarrow C) \wedge ((C \wedge D) \rightarrow \perp) \wedge (\top \rightarrow B).$
- ▶ $(\top \rightarrow A) \wedge (C \rightarrow D) \wedge ((A \wedge B) \rightarrow C) \wedge ((C \wedge D) \rightarrow \perp) \wedge (\top \rightarrow B).$

The Horn Algorithm

The Horn algorithm concludes **Sat** iff H is satisfiable.

Complexity of Horn

- ▶ Given a Horn formula ψ with n propositions, how many times do you have to read ψ ?
- ▶ Step 1: Read once
- ▶ Step 2: Read at most n times
- ▶ Step 3: Read once

2-CNF

- ▶ 2-CNF : CNF where each clause has at most 2 literals.

$$(\neg p \vee q) \wedge p \wedge (r \vee \neg q) \wedge (\neg r \vee p)$$